src/Parsers/BooleanBaseTypes.v
@@ -1,0 +1,61 @@
+(** * Definition of a boolean-returning CFG parser-recognizer *)
+Require Import Coq.Lists.List Coq.Program.Program Coq.Classes.RelationClasses Coq.Strings.String.
+Require Import Parsers.BaseTypes Parsers.ContextFreeGrammar.
+Require Import Parsers.MinimalParse.
+
+Local Coercion is_true : bool >-> Sortclass.
+
+Local Open Scope string_like_scope.
+
+Section general.
+  Context {CharType} {String : string_like CharType} {G : grammar CharType}.
+
+  Class boolean_parser_dataT :=
+    { predata :> parser_computational_predataT;
+      split_stateT : String -> Type;
+      data' :> _ := {| BaseTypes.predata := predata ; BaseTypes.split_stateT := fun _ _ _ => split_stateT |};
+      split_string_for_production
+      : forall it its,
+          StringWithSplitState String split_stateT
+          -> list (StringWithSplitState String split_stateT * StringWithSplitState String split_stateT);
+      split_string_for_production_correct
+      : forall it its (str : StringWithSplitState String split_stateT),
+          let P f := List.Forall f (split_string_for_production it its str) in
+          P (fun s1s2 =>
+               (fst s1s2 ++ snd s1s2 =s str) = true);
+      premethods :> parser_computational_dataT'
+      := @Build_parser_computational_dataT'
+           _ String data'
+           (fun _ _ => split_string_for_production)
+           (fun _ _ => split_string_for_production_correct) }.
+
+  Definition split_list_completeT `{data : boolean_parser_dataT}
+             {str0 valid}
+             (str : StringWithSplitState String split_stateT) (pf : str ≤s str0)
+             (split_list : list (StringWithSplitState String split_stateT * StringWithSplitState String split_stateT))
+             (it : item CharType) (its : production CharType)
+    := ({ s1s2 : String * String
+                 & (fst s1s2 ++ snd s1s2 =s str)
+                   * (minimal_parse_of_item _ G initial_nonterminals_data is_valid_nonterminal remove_nonterminal str0 valid (fst s1s2) it)
+                   * (minimal_parse_of_production _ G initial_nonterminals_data is_valid_nonterminal remove_nonterminal str0 valid (snd s1s2) its) }%type)
+       -> ({ s1s2 : StringWithSplitState String split_stateT * StringWithSplitState String split_stateT
+                    & (In s1s2 split_list)
+                      * (minimal_parse_of_item _ G initial_nonterminals_data is_valid_nonterminal remove_nonterminal str0 valid (fst s1s2) it)
+                      * (minimal_parse_of_production _ G initial_nonterminals_data is_valid_nonterminal remove_nonterminal str0 valid (snd s1s2) its) }%type).
+
+  Class boolean_parser_completeness_dataT' `{data : boolean_parser_dataT} :=
+    { remove_nonterminal_1
+      : forall ls ps ps',
+          is_valid_nonterminal (remove_nonterminal ls ps) ps' = true
+          -> is_valid_nonterminal ls ps' = true;
+      remove_nonterminal_2
+      : forall ls ps ps',
+          is_valid_nonterminal (remove_nonterminal ls ps) ps' = false
+          <-> is_valid_nonterminal ls ps' = false \/ ps = ps';
+      split_string_for_production_complete
+      : forall str0 valid str pf it its, @split_list_completeT _ str0 valid str pf (split_string_for_production it its str) it its }.
+
+  Class boolean_parser_correctness_dataT :=
+    { data :> boolean_parser_dataT;
+      cdata' :> boolean_parser_completeness_dataT' }.
+End general.
