src/Parsers/Splitters/BruteForce.v
@@ -1,0 +1,126 @@
+(** * Definition of a boolean-returning CFG parser-recognizer *)
+Require Import Coq.Lists.List Coq.Strings.String.
+Require Import Parsers.ContextFreeGrammar.
+Require Import Parsers.BaseTypes Parsers.BooleanBaseTypes.
+Require Import Parsers.Splitters.RDPList.
+Require Import Common.
+
+Set Implicit Arguments.
+Local Open Scope string_like_scope.
+
+Local Coercion is_true : bool >-> Sortclass.
+
+Definition String_with_no_state {CharType} (String : string_like CharType) := StringWithSplitState String (fun _ => True).
+
+Definition default_String_with_no_state {CharType} (String : string_like CharType) (s : String) : String_with_no_state String
+  := {| string_val := s ; state_val := I |}.
+
+Coercion default_string_with_no_state (s : string) : String_with_no_state string_stringlike
+  := default_String_with_no_state string_stringlike s.
+
+Identity Coercion unfold_String_with_no_state : String_with_no_state >-> StringWithSplitState.
+
+Section brute_force_splitter.
+  Fixpoint make_all_single_splits' (str : string) : list (String_with_no_state string_stringlike * String_with_no_state string_stringlike)
+    := ((""%string : String_with_no_state string_stringlike),
+        (str : String_with_no_state string_stringlike))
+         ::(match str with
+              | ""%string => nil
+              | String.String ch str' =>
+                map (fun p : String_with_no_state string_stringlike * String_with_no_state string_stringlike
+                     => ((String.String ch (string_val (fst p)) : String_with_no_state string_stringlike),
+                         snd p))
+                    (make_all_single_splits' str')
+            end).
+
+  Definition make_all_single_splits (str : String_with_no_state string_stringlike)
+    := make_all_single_splits' (string_val str).
+
+  Lemma make_all_single_splits_correct_eq (str : String_with_no_state string_stringlike)
+  : List.Forall (fun strs : String_with_no_state string_stringlike * String_with_no_state string_stringlike
+                 => string_val (fst strs) ++ string_val (snd strs) = string_val str)%string (make_all_single_splits str).
+  Proof.
+    destruct str as [str ?].
+    induction str; simpl in *; constructor; auto.
+    apply Forall_map.
+    unfold compose; simpl in *.
+    revert IHstr; apply Forall_impl; intros.
+    subst; trivial.
+  Qed.
+
+  Local Opaque string_dec.
+  Lemma make_all_single_splits_correct_seq (str : String_with_no_state string_stringlike)
+  : List.Forall (fun strs : String_with_no_state string_stringlike * String_with_no_state string_stringlike
+                 => (fst strs ++ snd strs =s str) = true)%string_like (make_all_single_splits str).
+  Proof.
+    destruct str as [str ?].
+    induction str; simpl; constructor; simpl; auto.
+    { rewrite string_dec_refl; reflexivity. }
+    { apply Forall_map.
+      unfold compose; simpl.
+      revert IHstr; apply Forall_impl; intros.
+      match goal with H : (_ =s _) = true |- _ => apply bool_eq_correct in H end.
+      simpl in *; subst; rewrite string_dec_refl; reflexivity. }
+  Qed.
+
+  Lemma make_all_single_splits_correct_str_le (str : String_with_no_state string_stringlike)
+  : List.Forall (fun strs : String_with_no_state string_stringlike * String_with_no_state string_stringlike
+                 => fst strs ≤s str /\ snd strs ≤s str)%string (make_all_single_splits str).
+  Proof.
+    generalize (make_all_single_splits_correct_eq str).
+    apply Forall_impl.
+    destruct str as [str ?]; simpl.
+    intros; subst; split;
+    first [ apply str_le1_append
+          | apply str_le2_append ].
+  Qed.
+
+  Local Hint Resolve NPeano.Nat.lt_lt_add_l NPeano.Nat.lt_lt_add_r NPeano.Nat.lt_add_pos_r NPeano.Nat.lt_add_pos_l : arith.
+  Local Hint Resolve str_le1_append str_le2_append.
+
+  Context (G : grammar Ascii.ascii).
+
+  Global Instance brute_force_premethods : @parser_computational_dataT' _ string_stringlike (@rdp_list_data' _ _ G)
+    := { split_string_for_production str0 valid it its := make_all_single_splits;
+         split_string_for_production_correct str0 valid it its := make_all_single_splits_correct_seq }.
+
+  Global Instance brute_force_data : @boolean_parser_dataT _ string_stringlike
+    := { predata := @rdp_list_predata _ G;
+         split_stateT str := True;
+         split_string_for_production it its := make_all_single_splits;
+         split_string_for_production_correct it its := make_all_single_splits_correct_seq }.
+
+  Lemma make_all_single_splits_complete_helper
+  : forall (str : String_with_no_state string_stringlike)
+           (s1s2 : String_with_no_state string_stringlike * String_with_no_state string_stringlike),
+      fst s1s2 ++ snd s1s2 =s str -> In s1s2 (make_all_single_splits str).
+  Proof.
+    intros [str [] ] [ [s1 [] ] [s2 [] ] ] H.
+    apply bool_eq_correct in H; simpl in *; subst.
+    revert s2.
+    induction s1; simpl in *.
+    { intros.
+      destruct s2; left; simpl; reflexivity. }
+    { intros; right.
+      refine (@in_map _ _ _ _ ({| string_val := s1 |}, {| string_val := s2 |}) _).
+      apply IHs1. }
+  Qed.
+
+  Lemma make_all_single_splits_complete
+  : forall G str0 valid str pf it its, @split_list_completeT _ string_stringlike G brute_force_data str0 valid str pf (@make_all_single_splits str) it its.
+  Proof.
+    intros; hnf.
+    intros [ [s1 s2] [ [ p1 p2 ] p3 ] ].
+    exists ({| string_val := s1 ; state_val := I |}, {| string_val := s2 ; state_val := I |}).
+    abstract (
+        repeat split; try assumption;
+        apply make_all_single_splits_complete_helper;
+        assumption
+      ).
+  Defined.
+
+  Global Instance brute_force_cdata : @boolean_parser_completeness_dataT' _ _ G brute_force_data
+    := { remove_nonterminal_1 := rdp_list_remove_nonterminal_1;
+         remove_nonterminal_2 := rdp_list_remove_nonterminal_2;
+         split_string_for_production_complete := @make_all_single_splits_complete G }.
+End brute_force_splitter.
