src/Parsers/Splitters/RDPList.v
@@ -1,0 +1,121 @@
+(** * Definition of the part of boolean-returning CFG parser-recognizer that instantiates things to lists *)
+Require Import Coq.Lists.List Coq.Strings.String Coq.Arith.Wf_nat.
+Require Import Parsers.ContextFreeGrammar.
+Require Import Parsers.BaseTypes Parsers.BooleanBaseTypes.
+
+Set Implicit Arguments.
+Local Open Scope string_like_scope.
+
+Section recursive_descent_parser_list.
+  Context {CharType} {String : string_like CharType} {G : grammar CharType}.
+  Definition rdp_list_nonterminals_listT : Type := list string.
+  Definition rdp_list_is_valid_nonterminal : rdp_list_nonterminals_listT -> string -> bool
+    := fun ls nt => if in_dec string_dec nt ls then true else false.
+  Definition rdp_list_remove_nonterminal : rdp_list_nonterminals_listT -> string -> rdp_list_nonterminals_listT
+    := fun ls nt =>
+         filter (fun x => if string_dec nt x then false else true) ls.
+
+  Definition rdp_list_nonterminals_listT_R : rdp_list_nonterminals_listT -> rdp_list_nonterminals_listT -> Prop
+    := ltof _ (@List.length _).
+  Lemma filter_list_dec {T} f (ls : list T) : List.length (filter f ls) <= List.length ls.
+  Proof.
+    induction ls; trivial; simpl in *.
+    repeat match goal with
+             | [ |- context[if ?a then _ else _] ] => destruct a; simpl in *
+             | [ |- S _ <= S _ ] => solve [ apply Le.le_n_S; auto ]
+             | [ |- _ <= S _ ] => solve [ apply le_S; auto ]
+           end.
+  Qed.
+  Lemma rdp_list_remove_nonterminal_dec : forall ls prods,
+                                            @rdp_list_is_valid_nonterminal ls prods = true
+                                            -> @rdp_list_nonterminals_listT_R (@rdp_list_remove_nonterminal ls prods) ls.
+  Proof.
+    intros.
+    unfold rdp_list_is_valid_nonterminal, rdp_list_nonterminals_listT_R, rdp_list_remove_nonterminal, ltof in *.
+    edestruct in_dec; [ | discriminate ].
+    match goal with
+      | [ H : In ?prods ?ls |- context[filter ?f ?ls] ]
+        => assert (~In prods (filter f ls))
+    end.
+    { intro H'.
+      apply filter_In in H'.
+      destruct H' as [? H'].
+      edestruct string_dec; congruence. }
+    { match goal with
+        | [ |- context[filter ?f ?ls] ] => generalize dependent f; intros
+      end.
+      induction ls; simpl in *; try congruence.
+      repeat match goal with
+               | [ |- context[if ?x then _ else _] ] => destruct x; simpl in *
+               | [ H : _ \/ _ |- _ ] => destruct H
+               | _ => progress subst
+               | [ H : ~(_ \/ _) |- _ ] => apply Decidable.not_or in H
+               | [ H : _ /\ _ |- _ ] => destruct H
+               | [ H : ?x <> ?x |- _ ] => exfalso; apply (H eq_refl)
+               | _ => apply Lt.lt_n_S
+               | _ => apply Le.le_n_S
+               | _ => apply filter_list_dec
+               | [ H : _ -> _ -> ?G |- ?G ] => apply H; auto
+             end. }
+  Qed.
+  Lemma rdp_list_ntl_wf : well_founded rdp_list_nonterminals_listT_R.
+  Proof.
+    unfold rdp_list_nonterminals_listT_R.
+    intro.
+    apply well_founded_ltof.
+  Defined.
+
+  Lemma rdp_list_remove_nonterminal_1
+  : forall ls ps ps',
+      rdp_list_is_valid_nonterminal (rdp_list_remove_nonterminal ls ps) ps' = true
+      -> rdp_list_is_valid_nonterminal ls ps' = true.
+  Proof.
+    unfold rdp_list_is_valid_nonterminal, rdp_list_remove_nonterminal.
+    repeat match goal with
+             | _ => exfalso; congruence
+             | _ => reflexivity
+             | [ |- appcontext[if ?E then _ else _] ] => destruct E
+             | _ => intro
+             | [ H : In _ (filter _ _) |- _ ] => apply filter_In in H
+             | [ H : _ /\ _ |- _ ] => destruct H
+             | [ H : ?T, H' : ~?T |- _ ] => destruct (H' H)
+           end.
+  Qed.
+
+  Lemma rdp_list_remove_nonterminal_2
+  : forall ls ps ps',
+      rdp_list_is_valid_nonterminal (rdp_list_remove_nonterminal ls ps) ps' = false
+      <-> rdp_list_is_valid_nonterminal ls ps' = false \/ ps = ps'.
+  Proof.
+    unfold rdp_list_is_valid_nonterminal, rdp_list_remove_nonterminal.
+    repeat match goal with
+             | _ => exfalso; congruence
+             | _ => reflexivity
+             | _ => progress subst
+             | _ => intro
+             | [ H : context[In _ (filter _ _)] |- _ ] => rewrite filter_In in H
+             | [ H : _ /\ _ |- _ ] => destruct H
+             | [ H : ?T, H' : ~?T |- _ ] => destruct (H' H)
+             | [ |- true = false \/ _ ] => right
+             | [ |- ?x = ?x \/ _ ] => left; reflexivity
+             | [ H : ~(_ /\ ?x = ?x) |- _ ] => specialize (fun y => H (conj y eq_refl))
+             | [ H : _ \/ _ |- _ ] => destruct H
+             | [ |- _ <-> _ ] => split
+             | [ H : appcontext[if ?E then _ else _] |- _ ] => destruct E
+             | [ |- appcontext[if ?E then _ else _] ] => destruct E
+           end.
+  Qed.
+
+  Global Instance rdp_list_predata : parser_computational_predataT
+    := { nonterminals_listT := rdp_list_nonterminals_listT;
+         initial_nonterminals_data := Valid_nonterminals G;
+         is_valid_nonterminal := rdp_list_is_valid_nonterminal;
+         remove_nonterminal := rdp_list_remove_nonterminal;
+         nonterminals_listT_R := rdp_list_nonterminals_listT_R;
+         remove_nonterminal_dec := rdp_list_remove_nonterminal_dec;
+         ntl_wf := rdp_list_ntl_wf }.
+
+  Global Instance rdp_list_data' : @parser_computational_types_dataT _ String
+    := { predata := rdp_list_predata;
+         split_stateT := fun _ _ _ _ => True }.
+End recursive_descent_parser_list.
